src/tactic/vampire/foo.sh
@@ -1,0 +1,5 @@
+#!/bin/sh
+
+echo $1
+
+echo "Hello"
