src/tactic/vampire/hello.pl
@@ -1,0 +1,6 @@
+#!/usr/bin/env swipl
+
+:- initialization(main, main).
+
+main(_) :-
+  print("Hello World!").
