src/tactic/vampire/rr.pl
@@ -1,0 +1,7 @@
+#!/usr/bin/env swipl
+
+:- initialization(main, main).
+
+main([Argv]) :-
+  split_string(Argv, " ", " ", Tks),
+  print(Tks).
