src/tactic/vampire/vampire.sh
@@ -1,5 +1,7 @@
 #!/bin/sh
 
-echo $1 > $2
+# echo $1 > $2
 
-vampire --avatar off $2
+# vampire --avatar off $2
+
+echo "Hello!"
